src/SemFacts.v
@@ -1,0 +1,25 @@
+Require Import Bool List String Peano_dec.
+Require Import Common FMap Syntax Semantics.
+
+Theorem refines_refl:
+  forall step sys, step # step |-- sys ⊑[id] sys.
+Proof.
+  unfold Refines; intros.
+  replace (map id hst) with hst; [assumption|].
+  clear; induction hst; simpl; auto.
+  f_equal; auto.
+Qed.
+
+Theorem refines_trans:
+  forall step1 step2 step3 s1 s2 s3 p q,
+    step1 # step2 |-- s1 ⊑[p] s2 ->
+    step2 # step3 |-- s2 ⊑[q] s3 ->
+    step1 # step3 |-- s1 ⊑[fun l => q (p l)] s3.
+Proof.
+  unfold Refines; intros.
+  specialize (H0 _ (H _ H1)).
+  replace (map _ hst) with (map q (map p hst)); [assumption|].
+  clear; induction hst; simpl; auto.
+  f_equal; auto.
+Qed.
+  
