src/SerialFacts.v
@@ -3,10 +3,9 @@ Require Import Permutation.
 Require Import Common FMap Syntax Semantics SemDet SemSeq Serial.
 
 Theorem sequential_step_seq:
-  forall sys tr,
-    Behavior step_det sys tr ->
-    Sequential (historyOf sys tr) ->
-    Behavior step_seq sys tr.
+  forall sys,
+    Serial step_det sys ->
+    step_det # step_seq |-- sys ⊑[id] sys.
 Proof.
 Admitted.
 
