src/Simulation.v
@@ -3,7 +3,7 @@ Require Import Common FMap Syntax Semantics.
 
 Section Simulation.
 
-  Variables (step: System -> State -> Label -> State -> Prop)
+  Variables (stepI stepS: System -> State -> Label -> State -> Prop)
             (sim: State -> State -> Prop)
             (p: BLabel -> BLabel).
 
@@ -15,14 +15,14 @@ Section Simulation.
     forall ist1 sst1,
       ist1 ≈ sst1 ->
       forall ilbl ist2,
-        step impl ist1 ilbl ist2 ->
+        stepI impl ist1 ilbl ist2 ->
         match toBLabel ilbl with
         | Some b =>
-          exists sst2 slbl, step spec sst1 slbl sst2 /\
+          exists sst2 slbl, stepS spec sst1 slbl sst2 /\
                             toBLabel slbl = Some (p b) /\
                             ist2 ≈ sst2
         | None =>
-          (exists sst2 slbl, step spec sst1 slbl sst2 /\
+          (exists sst2 slbl, stepS spec sst1 slbl sst2 /\
                              toBLabel slbl = None /\
                              ist2 ≈ sst2) \/
           ist2 ≈ sst1
@@ -34,10 +34,10 @@ Section Simulation.
     forall ist1 sst1,
       ist1 ≈ sst1 ->
       forall ihst ist2,
-        steps step impl ist1 ihst ist2 ->
+        steps stepI impl ist1 ihst ist2 ->
         exists sst2 shst,
           map p (behaviorOf ihst) = behaviorOf shst /\
-          steps step spec sst1 shst sst2 /\
+          steps stepS spec sst1 shst sst2 /\
           ist2 ≈ sst2.
   Proof.
     induction 2; simpl; intros;
@@ -63,7 +63,7 @@ Section Simulation.
 
   Hypothesis (Hsimi: sim (getStateInit impl) (getStateInit spec)).
 
-  Theorem simulation_implies_refinement: step |-- impl ⊑[p] spec.
+  Theorem simulation_implies_refinement: stepI # stepS |-- impl ⊑[p] spec.
   Proof.
     unfold Simulates, Refines; intros.
     inv H.
